Progress on admits

Dataflow/Memories.v
@@ -23,16 +23,6 @@ Module Type MEMORIES
        (Ids : IDS)
        (Op  : OPERATORS)
        (Import Syn : SYNTAX Ids Op).
-
-  (* definitions are needed in signature *)
-  Definition memory_eq (mems: PS.t) (eq: equation) : PS.t :=
-    match eq with
-    | EqFby x _ _ _ => PS.add x mems
-    | _ => mems
-    end.
-
-  Definition memories (eqs: list equation) : PS.t :=
-    List.fold_left memory_eq eqs PS.empty.
   
   (** ** Properties *)
 
